iris/ProofIlock.v
@@ -1079,7 +1079,8 @@ Section IlockLoad.
                     ind_res gfs bm ∗ inode_blocks gfs bm data))
                 ∨ ⌜bv_unsigned (di_type dn) = 0⌝))%I
       with "[Hpool HL]" as ">[HL Hrest]".
-    { rewrite /ipool_shape. iDestruct "Hpool" as "[Hal | Hmk]".
+    { rewrite /ipool_shape. iDestruct "Hpool" as "[Hal | [Hmk | Hoff]]";
+        last (iApply (InodeRegion.offlock_enabled_absurd with "Hoff")).
       - iDestruct "Hal" as (dn0 bm0 data0)
           "(%Hok0 & %Hdok0 & %Hddix0 & %Hdoc0 & %Hduq0 & Hdlk0 & Hdn & Hind & Hblk)".
         iMod (ireg_read ⊤ gi gfs inodestart nib inum dn0
